pulse/lib/pulse/core/PulseCore.MonotonicStateMonad.fst
@@ -1,18 +1,23 @@
 module PulseCore.MonotonicStateMonad
 open FStar.Preorder
+module PST = PulseCore.PreorderStateMonad
 module M = FStar.MSTTotal
 let mst (#s:Type u#s)
          (rel:FStar.Preorder.preorder s)
          (a:Type u#a)
          (pre:s -> prop)
          (post:s -> a -> s -> prop)
-  = s0:s { pre s0 }
-    -> Tot (
-        res:(a & s) {
-            post s0 res._1 res._2 /\
-            rel s0 res._2
-        }
-    )
+  = PST.pst a rel pre post
+
+let lift_pst
+    (#s:Type u#s)
+    (#rel:FStar.Preorder.preorder s)
+    (#a:Type u#a)
+    (#pre:s -> prop)
+    (#post:s -> a -> s -> prop)
+    (pst:PST.pst a rel pre post)
+: mst rel a pre post
+= pst
 
 assume (* to interoperate with a definition of a similar module in FStar.MSTTotal *)
 val reify_ (#s:Type u#2) (#rel:FStar.Preorder.preorder s)
@@ -33,22 +38,11 @@ let to_msttotal (#s:Type u#2) (rel:FStar.Preorder.preorder s)
 : M.MSTATETOT a s rel pre post
 = M.MSTATETOT?.reflect (fun s -> f s)
 
-let return x
-= fun s0 -> x, s0
-
-let bind f g
-= fun s0 ->
-    let x, s1 = f s0 in
-    g x s1
-
-let weaken f
-= fun s -> f s
-
-let get _
-= fun s -> s, s
-
-let put v
-= fun _  -> (), v
+let return = PST.return
+let bind = PST.bind
+let weaken = PST.weaken
+let get = PST.get
+let put = PST.put
 
 let witnessed p
 = unit
@@ -57,4 +51,6 @@ let witness p
 = fun s -> (), s
 
 let recall p w
-= fun s -> assume (p s); (), s
+= fun s ->
+    assume (p s);
+    (), s
